some experiments with gluing

theories/univalence.v
@@ -1,5 +1,6 @@
 From Theories Require Import category.
 From Theories Require Import translation_fib.
+From Theories Require Import transport.
 
 Set Primitive Projections.
 Set Universe Polymorphism.
@@ -36,3 +37,142 @@ unshelve econstructor.
 - simpl.
 Admitted. *)
 
+Inductive bool' : Set :=
+| true' : bool'
+| false' : bool'.
+
+Definition bool'R {p} : (forall q (α : q ≤ p), bool') -> SProp :=
+fun s => s ≡ fun q α => s p !.
+
+Definition bool'0 {p} : @El0 p Type0.
+Proof.
+unshelve refine (fun q α => mkYFT _ _ _ _).
+- unshelve refine (fun r β => bool').
+- unshelve refine (fun r β s => bool'R s).
+- unshelve refine (fun r β b e l le l' => _).
+  unshelve econstructor.
+  + unfold yt_funct ; simpl.
+    unshelve econstructor ; simpl.
+    apply falso.
+    apply sfalso.
+  + apply sfalso.
+Defined.
+
+Definition bool'1 {p} : @El1 p Type0 Type1 bool'0.
+Proof.
+unshelve refine (fun q α => _).
+reflexivity.
+Defined.
+
+Definition is_i1 {p} : p ≤ 1 -> bool.
+Admitted.
+
+Definition i1_is_i1 : (fun p => is_i1 (@i1 p)) ≡ fun _ => true.
+Admitted.
+
+Definition gluetest {p q} (α : q ≤ S p) :=
+  if is_i1 (antisquish ∘ α) then bool' else bool.
+
+Definition gluetest_funct {p q} {α : q ≤ S p} {r} (β : r ≤ q) :
+  gluetest α -> gluetest (α ∘ β).
+Admitted.
+
+Definition glue_test0 {p} :
+  @El0 (S p) (squish ⋅ Type0).
+Proof.
+refine (fun q α => _).
+unshelve econstructor.
+- refine (fun r β => _).
+  refine (gluetest (α ∘ β)).
+- refine (fun r β => _).
+  refine (fun s => s ≡ (fun r0 β0 => gluetest_funct β0 (s r !))).
+- unshelve refine (fun r β b e l le l' => _).
+  apply falso.
+Defined.
+
+Record yt_seq {p} (a b : forall q (α : q ≤ p), yt q) : SProp :=
+mkYTSEQ {
+  ytseq0 : (fun q (α : q ≤ p) => yt0 (a q α)) ≡ (fun q (α : q ≤ p) => yt0 (b q α)) ;
+  ytseq1 : (fun q (α : q ≤ p) r (β : r ≤ q) (s : forall r0 (β0 : r0 ≤ r), yt0 (b q α) r0 (β ∘ β0)) =>
+      yt1 (a q α) r β
+          (fun r0 (β0 : r0 ≤ r) => J_seq _ _ (fun X _ => X q α r0 (β ∘ β0)) (s r0 β0) _ (ssym ytseq0)))
+    ≡ (fun q (α : q ≤ p) => yt1 (b q α)) ;
+  }.
+
+Lemma trans {A : Type} {a b c : A} (e1 : a ≡ b) (e2 : b ≡ c) : a ≡ c.
+  Admitted.
+
+Lemma yt_seq_to_seq {p} (a b : forall q (α : q ≤ p), yt q) :
+  yt_seq a b -> a ≡ b.
+Proof.
+refine (fun Hab => _).
+pose proof (ytseq0 _ _ Hab) as Hab0.
+pose proof (ytseq1 _ _ Hab) as Hab1.
+change ((fun q (α : q ≤ p) =>
+  {| yt0 := yt0 (a q α) ;
+     yt1 := fun r (β : r ≤ q) (s : forall r0 (β0 : r0 ≤ r), yt0 (a q α) r0 (β ∘ β0)) => yt1 (a q α) r β (fun r0 (β0 : r0 ≤ r) => s r0 β0) |})
+≡
+(fun q (α : q ≤ p) =>
+  {| yt0 := yt0 (b q α) ;
+     yt1 := yt1 (b q α) |})).
+refine (J_seqs _ (fun q (α : q ≤ p) => yt0 (b q α))
+  (fun X E =>
+    (fun q (α : q ≤ p) => {|
+      yt0 := X q α ;
+      yt1 := fun r (β : r ≤ q) (s : forall r0 (β0 : r0 ≤ r), X q α r0 (β ∘ β0)) =>
+        yt1 (a q α) r β
+        (fun r0 (β0 : r0 ≤ r) => J_seq _ X (fun Y _ => Y q α r0 (β ∘ β0)) (s r0 β0) (fun q (α : q ≤ p) => yt0 (a q α)) (trans (ssym E) (ssym Hab0))) |})
+  ≡ (fun q (α : q ≤ p) => {| yt0 := yt0 (b q α) ; yt1 := yt1 (b q α) |}))
+  _ (fun q (α : q ≤ p) => yt0 (a q α)) (ssym Hab0)).
+refine (J_seqs _ _ (fun X _ => (fun q (α : q ≤ p) =>
+  {| yt0 := yt0 (b q α) ;
+     yt1 := X q α |}) ≡ b) _ _ (ssym Hab1)).
+reflexivity.
+Defined.
+
+Record yft_seq {p} (a b : forall q (α : q ≤ p), yft q) : SProp :=
+mkYFTSEQ {
+  yftseq0 : (fun q (α : q ≤ p) => yft0 (a q α)) ≡ (fun q (α : q ≤ p) => yft0 (b q α)) ;
+  yftseq1 : (fun q (α : q ≤ p) r (β : r ≤ q) (s : forall r0 (β0 : r0 ≤ r), yft0 (b q α) r0 (β ∘ β0)) =>
+      yft1 (a q α) r β
+          (fun r0 (β0 : r0 ≤ r) => J_seq _ _ (fun X _ => X q α r0 (β ∘ β0)) (s r0 β0) _ (ssym yftseq0)))
+    ≡ (fun q (α : q ≤ p) => yft1 (b q α)) ;
+  }.
+
+Goal ~ (~ (forall P : Prop, P \/ (~ P))).
+intro s.
+
+Lemma test {p} : 
+  yft_seq (side_1 ⋅ (@glue_test0 p)) (bool'0).
+Proof.
+unshelve econstructor.
+- change ((fun q (α : q ≤ p) r (β : r ≤ q) => if is_i1 (@i1 r) then bool' else bool) ≡ (fun q (α : q ≤ p) r (β : r ≤ q) => bool')).
+  refine (J_seqs (nat -> bool) (fun _ => true) (fun X _ => (fun q (α : q ≤ p) r (β : r ≤ q) => if X r then bool' else bool) ≡ _) (srefl _) _ (ssym i1_is_i1)).
+- simpl. unfold bool'R. 
+  assert (let x := (fun y => y) bool in x) as H. admit.
+  cbv zeta in H.
+ (* assuming is_i1 (i1) reduces to true, that reduces to the following *)
+ assert ((fun q (α : q ≤ p) r (β : r ≤ q) (s : forall r0 (β0 : r0 ≤ r), bool') =>
+    s ≡ (fun r0 (β0 : r0 ≤ r) => gluetest_funct β0 (s r !)))
+  ≡
+  (fun q (α : q ≤ p) r (β : r ≤ q) (s : forall r0 (β0 : r0 ≤ r), bool') =>
+    s ≡ (fun r0 (β0 : r0 ≤ r) => s r !))).
+
+
+
+unshelve econstructor.
+  + refine (fun r0 β0 => _).
+    exact (if (is_i1 (antisquish ∘ β ∘ β0)) then bool' else bool).
+  + refine (fun r0 β0 => _).
+    admit.
+
+    apply falso.
+- refine (fun r β => _). unshelve
+  (itype r0 Type bool bool').
+
+Definition univ_test0 {p} :
+  @El0 p (eq0 Type0 Type1 bool0 bool1 bool'0 bool'1).
+Proof.
+refine (fun q α => _).
+unshelve econstructor.
+- refine (fun r β => _).
